{
  "@context": {
    "iot": "http://iotschema.org/",
    "owl": "http://www.w3.org/2002/07/owl#",
    "qudt": "http://qudt.org/1.1/schema/qudt#",
    "rdf": "http://www.w3.org/1999/02/22-rdf-syntax-ns#",
    "rdfs": "http://www.w3.org/2000/01/rdf-schema#",
    "schema": "http://schema.org/",
    "xsd": "http://www.w3.org/2001/XMLSchema#",
	"dct": "http://purl.org/dc/terms/"
  },
  "@graph": [
    {
		"@id": "iot:TemperatureUnit",
		"@type": "rdfs:Class",
		"rdfs:comment": "An enumeration of temperature units.",
		"rdfs:label": "TemperatureUnit",
		"rdfs:subClassOf": {
		"@id": "schema:Enumeration"
		}
	},
    {
		"@id": "iot:Celsius",
		"@type": "iot:TemperatureUnit",
		"rdfs:comment": "unit of the temperature of which the scale is defined by two fixe-points, the temperatures of freezing and boiling point of water at normal pressure (air pressure of 1 013,25 hPa)",
		"rdfs:label": "째C",
		"iot:reference": "0112/2///62720#UAA033#001",
		"dct:source": "http://data.nasa.gov/qudt/owl/unit#DegreeCelsius"
	},
    {
		"@id": "iot:Kelvin",
		"@type": "iot:TemperatureUnit",
		"rdfs:comment": "unit of thermodynamic temperature is the fraction 1/273,16 of the thermodynamic temperature of the triple point of water",
		"rdfs:label": "K",
		"iot:reference" : "0112/2///62720#UAA185#001",
		"dct:source": "http://data.nasa.gov/qudt/owl/unit#Kelvin"
    },
	{
		"@id": "iot:Fahrenheit",
		"@type": "iot:TemperatureUnit",
		"rdfs:comment": "unit of temperature according to the temperature of the freezing and boiling point of water (32 째F and 212 째F)",
		"rdfs:label": "째F",
		"iot:reference" : "0112/2///62720#UAA039#001",
		"dct:source": "http://data.nasa.gov/qudt/owl/unit#DegreeFahrenheit"
    },
	{
		"@id": "iot:TimeUnitType",
		"@type": "rdfs:Class",
		"rdfs:comment": "An enumeration of time unit.",
		"rdfs:label": "TimeUnitType",
		"rdfs:subClassOf": {
			"@id": "schema:Enumeration"
		}
	},
    {
		"@id": "iot:Second",
		"@type": "iot:TimeUnitType",
		"rdfs:comment": "Second Time Unit",
		"rdfs:label": "s",
	    "iot:reference" : "0112/2///62720#UAA972#001",
	    "dct:source": "http://data.nasa.gov/qudt/owl/unit#SecondTime"
	},
    {
		"@id": "iot:Minute",
		"@type": "iot:TimeUnitType",
		"rdfs:comment": "Minute Time Unit",
		"rdfs:label": "min",
	    "iot:reference" : "0112/2///62720#UAA842#001",
	    "dct:source": "http://data.nasa.gov/qudt/owl/unit#MinuteTime"
	},
    {
		"@id": "iot:Hour",
		"@type": "iot:TimeUnitType",
		"rdfs:comment": "Hour Time Unit",
		"rdfs:label": "h",
	    "iot:reference" : "0112/2///62720#UAA407#001",
	    "dct:source": "http://data.nasa.gov/qudt/owl/unit#Hour"
	},
    {
		"@id": "iot:Lux",
		"@type": "iot:IlluminanceUnit",
		"rdfs:comment": "Illuminance Unit",
		"rdfs:label": "lx",
	    "iot:reference" : "0112/2///62720#UAA723#001",
	    "dct:source": "http://qudt.org/vocab/unit#Lux"
	},
	{
		"@id": "iot:LevelUnit",
		"@type": "rdfs:Class",
		"rdfs:comment": "An enumeration of level units.",
		"rdfs:label": "LevelUnit",
		"rdfs:subClassOf": {
		"@id": "schema:Enumeration"
		}
	},
    {
		"@id": "iot:Percent",
		"@type": "iot:LevelUnit",
		"@type": "iot:GasInAirConcentrationUnit",
		"rdfs:comment": "Unit of measurement for level or concentration.",
		"rdfs:label": "%",
	    "iot:reference" : "0112/2///62720#UAA000#001",
	    "dct:source": "http://qudt.org/vocab/unit#Percent"
	},
    {
		"@id": "iot:Millimetre",
		"@type": "iot:LevelUnit",
		"rdfs:comment": "Unit of measurement in millimetre",
		"rdfs:label": "mm",
	    "iot:reference" : "0112/2///62720#UAA862#001"
	},
    {
		"@id": "iot:Centimetre",
		"@type": "iot:LevelUnit",
		"rdfs:comment": "Unit of measurement in centimetre",
		"rdfs:label": "cm",
	    "iot:reference" : "0112/2///62720#UAA375#001",
	    "dct:source": "http://qudt.org/vocab/unit#Centimeter"
	},
	{
		"@id": "iot:DensityUnit",
		"@type": "rdfs:Class",
		"rdfs:comment": "An enumeration of density units.",
		"rdfs:label": "DensityUnit",
		"rdfs:subClassOf": {
		"@id": "schema:Enumeration"
		}
	},
    {
		"@id": "iot:KilogramPerCubicMeter",
		"@type": "iot:DensityUnit",
		"rdfs:comment": "unit of the density of liquid",
		"rdfs:label": "kg/m3",
		"iot:reference": "0112/2///62720#UAA619#001",
		"dct:source": "http://data.nasa.gov/qudt/owl/unit#KilogramPerCubicMeter"
	},
    {
		"@id": "iot:PressureUnit",
		"@type": "rdfs:Class",
		"rdfs:comment": "An enumeration of pressure units.",
		"rdfs:label": "PressureUnit",
		"rdfs:subClassOf": {
		"@id": "schema:Enumeration"
		}
	},
    {
		"@id": "iot:Pascal",
		"@type": "iot:PressureUnit",
		"rdfs:comment": "The pascal (symbol: Pa) is the SI derived unit of pressure used to quantify internal pressure, stress, Young's modulus and ultimate tensile strength. It is defined as one newton per square metre.",
		"rdfs:label": "Pa",
		"iot:reference": "0112/2///62720#UAA258#001",
		"dct:source": "http://data.nasa.gov/qudt/owl/unit#Pascal"
	},
    {
		"@id": "iot:Bar",
		"@type": "iot:PressureUnit",
		"rdfs:comment": "The bar (symbol: bar) is a metric unit of pressure, but is not approved as part of the International System of Units (SI).",
		"rdfs:label": "bar",
		"iot:reference": "0112/2///62720#UAA323#001",
		"dct:source": "http://data.nasa.gov/qudt/owl/unit#Bar"
	},
    {
		"@id": "iot:FlowRateUnit",
		"@type": "rdfs:Class",
		"rdfs:comment": "An enumeration of flow rate units.",
		"rdfs:label": "FlowRateUnit",
		"rdfs:subClassOf": {
		"@id": "schema:Enumeration"
		}
	},
    {
		"@id": "iot:GallonsPerMinute",
		"@type": "iot:FlowRateUnit",
		"rdfs:comment": "unit of measurement of liquid flow rate",
		"rdfs:label": "gal/min",
		"dct:source":"http://data.nasa.gov/qudt/owl/unit#GallonUSPerMinute"
	},
    {
		"@id": "iot:LitrePerMinute",
		"@type": "iot:FlowRateUnit",
		"rdfs:comment": "Unit of measurement of flow rate of a substance",
		"rdfs:label": "l/min",
		"iot:reference": "0112/2///62720#UAA659#001"
	},
	{
		"@id": "iot:Decibel",
		"@type": "iot:SoundPressureUnit",
		"rdfs:comment": "Sound Pressure Unit",
		"rdfs:label": "dB",
		"iot:reference" : "0112/2///62720#UAA409#001",
		"dct:source": "http://qudt.org/vocab/unit#Decibel"
	},
	{
		"@id": "iot:GasInAirConcentrationUnit",
		"@type": "rdfs:Class",
		"rdfs:comment": "An enumeration of units for concentration of gas in the air, e.g., concentration of carbon dioxide (CO2) in ambient air.",
		"rdfs:label": "GasInAirConcentrationUnit",
		"rdfs:subClassOf": {
		"@id": "schema:Enumeration"
		}
	},
	{
		"@id": "iot:PartsPerMillion",
		"@type": "iot:GasInAirConcentrationUnit",
		"rdfs:comment": "The unit of concentration of gas in the air, e.g., concentration of carbon dioxide (CO2) in ambient air.",
		"rdfs:label": "ppm"
	},	
	{
		"@id": "iot:ApparentPowerUnit",
		"@type": "rdfs:Class",
		"rdfs:comment": "An enumeration of apparent power units.",
		"rdfs:label": "ApparentPowerUnit",
		"rdfs:subClassOf": {
		"@id": "schema:Enumeration"
		}
	},
	{
		"@id": "iot:VoltAmpere",
		"@type": "iot:ApparentPowerUnit",
		"rdfs:comment": "The unit of the apparent power.",
		"rdfs:label": "VA",
		"iot:reference": "0112/2///62720#UAA298#001"
	},
	{
		"@id": "iot:KiloVoltAmpere",
		"@type": "iot:ApparentPowerUnit",
		"rdfs:comment": "The unit of the apparent power, expressed in kilo (one thousand) as a decimal unit prefix.",
		"rdfs:label": "kVA",
		"iot:reference": "0112/2///62720#UAA581#001"
	},
	{
		"@id": "iot:MegaVoltAmpere",
		"@type": "iot:ApparentPowerUnit",
		"rdfs:comment": "The unit of the apparent power, expressed in mega (one million) as a decimal unit prefix.",
		"rdfs:label": "MVA",
		"iot:reference": "0112/2///62720#UAA222#001"
	},
	{
		"@id": "iot:GigaVoltAmpere",
		"@type": "iot:ApparentPowerUnit",
		"rdfs:comment": "The unit of the apparent power, expressed in giga (one billion) as a decimal unit prefix.",
		"rdfs:label": "GVA", 
		"iot:reference": "0112/2///62720#UAB534#001"
	},
	{
		"@id": "iot:ActivePowerUnit",
		"@type": "rdfs:Class",
		"rdfs:comment": "An enumeration of active power units.",
		"rdfs:label": "ActivePowerUnit",
		"rdfs:subClassOf": {
		"@id": "schema:Enumeration"
		}
	},
	{
		"@id": "iot:Watt",
		"@type": "iot:ActivePowerUnit",
		"rdfs:comment": "The unit of the active power.",
		"rdfs:label": "W",
		"dct:source": "http://www.qudt.org/qudt/owl/1.0.0/unit/Instances.html#Watt",
		"iot:reference": "0112/2///62720#UAA306#001"
	},
	{
		"@id": "iot:KiloWatt",
		"@type": "iot:ActivePowerUnit",
		"rdfs:comment": "The unit of the active power, expressed in kilo (one thousand) as a decimal unit prefix.",
		"rdfs:label": "kW",
		"iot:reference": "0112/2///62720#UAA583#001"
	},
	{
		"@id": "iot:MegaWatt",
		"@type": "iot:ActivePowerUnit",
		"rdfs:comment": "The unit of the active power, expressed in mega (one million) as a decimal unit prefix.",
		"rdfs:label": "MW",
		"iot:reference": "0112/2///62720#UAA224#001"
	},
	{
		"@id": "iot:GigaWatt",
		"@type": "iot:ActivePowerUnit",
		"rdfs:comment": "The unit of the active power, expressed in giga (one billion) as a decimal unit prefix.",
		"rdfs:label": "GW",
		"iot:reference": "0112/2///62720#UAA154#001"
	},
	{
		"@id": "iot:ReactivePowerUnit",
		"@type": "rdfs:Class",
		"rdfs:comment": "An enumeration of reactive power units.",
		"rdfs:label": "ReactivePowerUnit",
		"rdfs:subClassOf": {
		"@id": "schema:Enumeration"
		}
	},
	{
		"@id": "iot:VoltAmpereReactive",
		"@type": "iot:ReactivePowerUnit",
		"rdfs:comment": "The unit of reactive power.",
		"rdfs:label": "var",
		"iot:reference": "0112/2///62720#UAB023#001"
	},
	{
		"@id": "iot:KiloVoltAmpereReactive",
		"@type": "iot:ReactivePowerUnit",
		"rdfs:comment": "The unit of reactive power, expressed in kilo (one thousand) as a decimal unit prefix.",
		"rdfs:label": "kvar",
		"iot:reference": "0112/2///62720#UAB195#001"
	},
	{
		"@id": "iot:MegaVoltAmpereReactive",
		"@type": "iot:ReactivePowerUnit",
		"rdfs:comment": "The unit of reactive power, expressed in mega (one million) as a decimal unit prefix.",
		"rdfs:label": "Mvar",
		"iot:reference": "0112/2///62720#UAB199#001"
	},
	{
		"@id": "iot:GigaVoltAmpereReactive",
		"@type": "iot:ReactivePowerUnit",
		"rdfs:comment": "The unit of reactive power, expressed in giga (one billion) as a decimal unit prefix.",
		"rdfs:label": "Gvar"
	},	
	{
		"@id": "iot:ElectricCurrentUnit",
		"@type": "rdfs:Class",
		"rdfs:comment": "An enumeration of electric current units.",
		"rdfs:label": "ElectricCurrentUnit",
		"rdfs:subClassOf": {
		"@id": "schema:Enumeration"
		}
	},
	{
		"@id": "iot:Ampere",
		"@type": "iot:ElectricCurrentUnit",
		"rdfs:comment": "The unit of electric current.",
		"rdfs:label": "A",
		"iot:reference": "0112/2///62720#UAA101#001",
		"dct:source": "http://www.qudt.org/qudt/owl/1.0.0/unit/Instances.html#Ampere"
	},
	{
		"@id": "iot:FemtoAmpere",
		"@type": "iot:ElectricCurrentUnit",
		"rdfs:comment": "The unit of electric current, expressed in a unit prefix meaning 'one 0.000000000000001'.",
		"rdfs:label": "fA",
		"iot:reference": "0112/2///62720#UAB638#001"
	},
	{
		"@id": "iot:PicoAmpere",
		"@type": "iot:ElectricCurrentUnit",
		"rdfs:comment": "The unit of electric current, expressed in a unit prefix meaning 'one trillionth'.",
		"rdfs:label": "pA",
		"iot:reference": "0112/2///62720#UAA928#001"
	},
	{
		"@id": "iot:NanoAmpere",
		"@type": "iot:ElectricCurrentUnit",
		"rdfs:comment": "The unit of electric current, expressed in a unit prefix meaning 'one billionth'.",
		"rdfs:label": "nA",
		"iot:reference": "0112/2///62720#UAA901#001"
	},
	{
		"@id": "iot:MicroAmpere",
		"@type": "iot:ElectricCurrentUnit",
		"rdfs:comment": "The unit of electric current, expressed in a unit prefix meaning 'one millionth'.",
		"rdfs:label": "쨉A",
		"iot:reference": "0112/2///62720#UAA057#001"
	},
	{
		"@id": "iot:MilliAmpere",
		"@type": "iot:ElectricCurrentUnit",
		"rdfs:comment": "The unit of electric current, expressed in a unit prefix meaning 'one thousandth'.",
		"rdfs:label": "mA",
		"iot:reference": "0112/2///62720#UAA775#001"
	},
	{
		"@id": "iot:KiloAmpere",
		"@type": "iot:ElectricCurrentUnit",
		"rdfs:comment": "The unit of electric current, expressed in a unit prefix meaning 'one thousand'.",
		"rdfs:label": "kA",
		"iot:reference": "0112/2///62720#UAA557#001"
	},
	{
		"@id": "iot:MegaAmpere",
		"@type": "iot:ElectricCurrentUnit",
		"rdfs:comment": "The unit of electric current, expressed in a unit prefix meaning 'one million'.",
		"rdfs:label": "MA",
		"iot:reference": "0112/2///62720#UAA202#001"
	},
	{
		"@id": "iot:GigaAmpere",
		"@type": "iot:ElectricCurrentUnit",
		"rdfs:comment": "The unit of electric current, expressed in a unit prefix meaning 'one billion'.",
		"rdfs:label": "GA"
	},
	{
		"@id": "iot:TeraAmpere",
		"@type": "iot:ElectricCurrentUnit",
		"rdfs:comment": "The unit of electric current, expressed in a unit prefix meaning 'one trillion'.",
		"rdfs:label": "TA",
		"iot:reference": "0112/2///62720#UAB640#001"
	},	
	{
		"@id": "iot:LineFrequencyUnit",
		"@type": "rdfs:Class",
		"rdfs:comment": "An enumeration of line frequency units.",
		"rdfs:label": "LineFrequencyUnit",
		"rdfs:subClassOf": {
		"@id": "schema:Enumeration"
		}
	},
	{
		"@id": "iot:Hertz",
		"@type": "iot:LineFrequencyUnit",
		"rdfs:comment": "The unit of line frequency.",
		"rdfs:label": "Hz",
		"iot:reference": "0112/2///62720#UAA170#001",
		"dct:source": "http://www.qudt.org/qudt/owl/1.0.0/unit/Instances.html#Hertz"
	},
	{
		"@id": "iot:Femtohertz",
		"@type": "iot:LineFrequencyUnit",
		"rdfs:comment": "The unit of line frequency, expressed in a unit prefix meaning 'one 0.000000000000001'.",
		"rdfs:label": "fHz"
	},
	{
		"@id": "iot:Picohertz",
		"@type": "iot:LineFrequencyUnit",
		"rdfs:comment": "The unit of line frequency, expressed in a unit prefix meaning 'one trillionth'.",
		"rdfs:label": "pHz"
	},
	{
		"@id": "iot:Nanoampere",
		"@type": "iot:LineFrequencyUnit",
		"rdfs:comment": "The unit of line frequency, expressed in a unit prefix meaning 'one billionth'.",
		"rdfs:label": "nHz"
	},
	{
		"@id": "iot:Microhertz",
		"@type": "iot:LineFrequencyUnit",
		"rdfs:comment": "The unit of line frequency, expressed in a unit prefix meaning 'one millionth'.",
		"rdfs:label": "쨉Hz"
	},
	{
		"@id": "iot:Millihertz",
		"@type": "iot:LineFrequencyUnit",
		"rdfs:comment": "The unit of line frequency, expressed in a unit prefix meaning 'one thousandth'.",
		"rdfs:label": "mHz",
		"iot:reference": "0112/2///62720#UAB698#001"
	},
	{
		"@id": "iot:KiloHertz",
		"@type": "iot:LineFrequencyUnit",
		"rdfs:comment": "The unit of line frequency, expressed in a unit prefix meaning 'one thousand'.",
		"rdfs:label": "kHz",
		"iot:reference": "0112/2///62720#UAA566#001",
		"dct:source": "http://www.qudt.org/qudt/owl/1.0.0/unit/Instances.html#KiloHertz"
	},
	{
		"@id": "iot:MegaHertz",
		"@type": "iot:LineFrequencyUnit",
		"rdfs:comment": "The unit of line frequency, expressed in a unit prefix meaning 'one million'.",
		"rdfs:label": "MHz",
		"iot:reference": "0112/2///62720#UAA209#001",
		"dct:source": "http://www.qudt.org/qudt/owl/1.0.0/unit/Instances.html#MegaHertz"
	},
	{
		"@id": "iot:GigaHertz",
		"@type": "iot:LineFrequencyUnit",
		"rdfs:comment": "The unit of line frequency, expressed in a unit prefix meaning 'one billion'.",
		"rdfs:label": "GHz",
		"iot:reference": "0112/2///62720#UAA150#001",
		"dct:source": "http://www.qudt.org/qudt/owl/1.0.0/unit/Instances.html#GigaHertz"
	},
	{
		"@id": "iot:TeraHertz",
		"@type": "iot:LineFrequencyUnit",
		"rdfs:comment": "The unit of line frequency, expressed in a unit prefix meaning 'one trillion'.",
		"rdfs:label": "THz",
		"iot:reference": "0112/2///62720#UAA287#001"
	},	
	{
		"@id": "iot:VoltageUnit",
		"@type": "rdfs:Class",
		"rdfs:comment": "An enumeration of voltage units.",
		"rdfs:label": "VoltageUnit",
		"rdfs:subClassOf": {
		"@id": "schema:Enumeration"
		}
	},
	{
		"@id": "iot:Volt",
		"@type": "iot:VoltageUnit",
		"rdfs:comment": "The unit of voltage.",
		"rdfs:label": "V",
		"iot:reference": "0112/2///62720#UAA296#001",
		"dct:source": "http://www.qudt.org/qudt/owl/1.0.0/unit/Instances.html#Volt"
	},
	{
		"@id": "iot:FemtoVolt",
		"@type": "iot:VoltageUnit",
		"rdfs:comment": "The unit of voltage, expressed in a unit prefix meaning 'one 0.000000000000001'.",
		"rdfs:label": "fV",
		"iot:reference": "0112/2///62720#UAC770#001"
	},
	{
		"@id": "iot:PicoVolt",
		"@type": "iot:VoltageUnit",
		"rdfs:comment": "The unit of voltage, expressed in a unit prefix meaning 'one trillionth'.",
		"rdfs:label": "pV",
		"iot:reference": "0112/2///62720#UAB363#001"
	},
	{
		"@id": "iot:NanoVolt",
		"@type": "iot:VoltageUnit",
		"rdfs:comment": "The unit of voltage, expressed in a unit prefix meaning 'one billionth'.",
		"rdfs:label": "nV",
		"iot:reference": "0112/2///62720#UAC771#001"
	},
	{
		"@id": "iot:MicroVolt",
		"@type": "iot:VoltageUnit",
		"rdfs:comment": "The unit of voltage, expressed in a unit prefix meaning 'one millionth'.",
		"rdfs:label": "쨉V",
		"iot:reference": "0112/2///62720#UAA078#001"
	},
	{
		"@id": "iot:MilliVolt",
		"@type": "iot:VoltageUnit",
		"rdfs:comment": "The unit of voltage, expressed in a unit prefix meaning 'one thousandth'.",
		"rdfs:label": "mV",
		"iot:reference": "0112/2///62720#UAA804#001"
	},
	{
		"@id": "iot:KiloVolt",
		"@type": "iot:VoltageUnit",
		"rdfs:comment": "The unit of voltage, expressed in a unit prefix meaning 'one thousand'.",
		"rdfs:label": "kV",
		"iot:reference": "0112/2///62720#UAA580#001"
	},
	{
		"@id": "iot:MegaVolt",
		"@type": "iot:VoltageUnit",
		"rdfs:comment": "The unit of voltage, expressed in a unit prefix meaning 'one million'.",
		"rdfs:label": "MV",
		"iot:reference": "0112/2///62720#UAA221#001"
	},
	{
		"@id": "iot:GigaVolt",
		"@type": "iot:VoltageUnit",
		"rdfs:comment": "The unit of voltage, expressed in a unit prefix meaning 'one billion'.",
		"rdfs:label": "GV",
		"iot:reference": "0112/2///62720#UAC772#001"
	},
	{
		"@id": "iot:TeraVolt",
		"@type": "iot:VoltageUnit",
		"rdfs:comment": "The unit of voltage, expressed in a unit prefix meaning 'one trillion'.",
		"rdfs:label": "TV",
		"iot:reference": "0112/2///62720#UAC773#001"
	},	
	{
		"@id": "iot:ApparentEnergyUnit",
		"@type": "rdfs:Class",
		"rdfs:comment": "An enumeration of apparent energy units.",
		"rdfs:label": "ApparentEnergyUnit",
		"rdfs:subClassOf": {
		"@id": "schema:Enumeration"
		}
	},
	{
		"@id": "iot:VoltAmpereHour",
		"@type": "iot:ApparentEnergyUnit",
		"rdfs:comment": "The unit of the apparent energy.",
		"rdfs:label": "VAh"
	},
	{
		"@id": "iot:KiloVoltAmpereHour",
		"@type": "iot:ApparentEnergyUnit",
		"rdfs:comment": "The unit of the apparent enregy, expressed in kilo (one thousand) as a decimal unit prefix.",
		"rdfs:label": "kVAh"
	},
	{
		"@id": "iot:MegaVoltAmpereHour",
		"@type": "iot:ApparentEnergyUnit",
		"rdfs:comment": "The unit of the apparent enregy, expressed in mega (one million) as a decimal unit prefix.",
		"rdfs:label": "MVAh"
	},
	{
		"@id": "iot:GigaVoltAmpereHour",
		"@type": "iot:ApparentEnergyUnit",
		"rdfs:comment": "The unit of the apparent enregy, expressed in giga (one billion) as a decimal unit prefix.",
		"rdfs:label": "GVAh"
	},
	{
		"@id": "iot:TeraVoltAmpereHours",
		"@type": "iot:ApparentPowerUnit",
		"rdfs:comment": "The unit of the apparent enregy, expressed in giga (one trillion) as a decimal unit prefix.",
		"rdfs:label": "TVAh"
	},
	{
		"@id": "iot:ActiveEnergyUnit",
		"@type": "rdfs:Class",
		"rdfs:comment": "An enumeration of active enregy units.",
		"rdfs:label": "ActiveEnergyUnit",
		"rdfs:subClassOf": {
		"@id": "schema:Enumeration"
		}
	},
	{
		"@id": "iot:WattHour",
		"@type": "iot:ActiveEnergyUnit",
		"rdfs:comment": "The unit of the active enregy.",
		"rdfs:label": "Wh",
		"dct:source": "http://www.qudt.org/qudt/owl/1.0.0/unit/Instances.html#Watthour",
		"iot:reference": "0112/2///62720#UAA308#001"
	},
	{
		"@id": "iot:KiloWattHour",
		"@type": "iot:ActiveEnergyUnit",
		"rdfs:comment": "The unit of the active enregy, expressed in kilo (one thousand) as a decimal unit prefix.",
		"rdfs:label": "kWh",
		"dct:source": "http://www.qudt.org/qudt/owl/1.0.0/unit/Instances.html#Kilowatthour",
		"iot:reference": "0112/2///62720#UAA584#001"
	},
	{
		"@id": "iot:MegaWattHour",
		"@type": "iot:ActiveEnergyUnit",
		"rdfs:comment": "The unit of the active enregy, expressed in mega (one million) as a decimal unit prefix.",
		"rdfs:label": "MWh",
		"iot:reference": "0112/2///62720#UAA225#001"
	},
	{
		"@id": "iot:GigaWattHour",
		"@type": "iot:ActiveEnergyUnit",
		"rdfs:comment": "The unit of the active enregy, expressed in giga (one billion) as a decimal unit prefix.",
		"rdfs:label": "GWh",
		"iot:reference": "0112/2///62720#UAA155#001"
	},
	{
		"@id": "iot:TeraWattHour",
		"@type": "iot:ActiveEnergyUnit",
		"rdfs:comment": "The unit of the active enregy, expressed in giga (one trillion) as a decimal unit prefix.",
		"rdfs:label": "TWh",
		"iot:reference": "0112/2///62720#UAA155#001"
	},
	{
		"@id": "iot:ReactiveEnergyUnit",
		"@type": "rdfs:Class",
		"rdfs:comment": "An enumeration of reactive enregy units.",
		"rdfs:label": "ReactiveEnergyUnit",
		"rdfs:subClassOf": {
		"@id": "schema:Enumeration"
		}
	},
	{
		"@id": "iot:VoltAmpereReactiveHour",
		"@type": "iot:ReactiveEnergyUnit",
		"rdfs:comment": "The unit of reactive enregy.",
		"rdfs:label": "varh"
	},
	{
		"@id": "iot:KiloVoltAmpereReactiveHour",
		"@type": "iot:ReactiveEnergyUnit",
		"rdfs:comment": "The unit of reactive enregy, expressed in kilo (one thousand) as a decimal unit prefix.",
		"rdfs:label": "kvarh",
		"iot:reference": "0112/2///62720#UAB195#001"
	},
	{
		"@id": "iot:MegaVoltAmpereReactiveHour",
		"@type": "iot:ReactiveEnergyUnit",
		"rdfs:comment": "The unit of reactive enregy, expressed in mega (one million) as a decimal unit prefix.",
		"rdfs:label": "Mvarh",
		"iot:reference": "0112/2///62720#UAB198#001"
	},
	{
		"@id": "iot:GigaVoltAmpereReactiveHour",
		"@type": "iot:ReactiveEnergyUnit",
		"rdfs:comment": "The unit of reactive enregy, expressed in giga (one billion) as a decimal unit prefix.",
		"rdfs:label": "Gvarh"
	},
	{
		"@id": "iot:TeraVoltAmpereReactiveHour",
		"@type": "iot:ReactiveEnergyUnit",
		"rdfs:comment": "The unit of the reactive enregy, expressed in giga (one trillion) as a decimal unit prefix.",
		"rdfs:label": "Tvarh"
	}
  ]
}
